### #10. Largest Common in String (Subsequence)

Given two strings text1 and text2, return the length of their longest common subsequence.

```
Input: text1 = "abcde", text2 = "ace" 
Output: 3
```

**CPP - DP (Recursion)**
```cpp
int matchSeq(string a, string b, int m, int n) {
	if (m == 0 || n == 0)
		return 0;

	if (a[m - 1] == b[n - 1])
		return 1 + matchSeq(a, b, m - 1, n - 1);

	return max(matchSeq(a, b, m - 1, n), matchSeq(a, b, m, n - 1));
}
```

**CPP (Tabulation) DP**
```cpp
int commonString(string a, string b, int m, int n) {
	int t[m + 1][n + 1];

	for (int i = 0; i < m + 1; i++)
		for (int j = 0; j < n + 1; j++)
			if (i == 0 || j == 0)
				t[i][j] = 0;
			else if (a[i - 1] == b[j - 1])
				t[i][j] = 1 + t[i - 1][j - 1];
			else
				t[i][j] = max(t[i - 1][j], t[i][j - 1]);

	return t[m][n];
}
```

**CPP - DP (Tabulation)**
```cpp
int matchSeq(string a, string b, int m, int n) {
	int t[m + 1][n + 1];

	for (int i = 0; i < m + 1; i++)
		for (int j = 0; j < n + 1; j++)
			if (i == 0 || j == 0)
				t[i][j] = 0;

	for (int i = 1; i < m + 1; i++)
		for (int j = 1; j < n + 1; j++)
			if (a[i - 1] == b[j - 1])
				t[i][j] = 1 + t[i - 1][j - 1];
			else
				t[i][j] = max(t[i - 1][j], t[i][j - 1]);

	return t[m][n];
}
```


### Largest Substring

**CPP**
```cpp
int countCommon(string a, string b, int m, int n) {
	int t[m + 1][n + 1];
	int best_count = 0;

	for (int i = 1; i < m + 1; i++)
		for (int j = 1; j < n + 1; j++)
			if (a[i - 1] == b[j - 1]) {
				t[i][j] = 1 + t[i - 1][j - 1];
				best_count = max(t[i][j], best_count);
			}
			else
				t[i][j] = 0;

	return best_count;
}
```
### Printing Longest Subtring

**CPP**
```cpp
string countCommon(string a, string b, int m, int n) {
	int t[m + 1][n + 1];
	int best_count = 0;

	for (int i = 1; i < m + 1; i++)
		for (int j = 1; j < n + 1; j++)
			if (a[i - 1] == b[j - 1]) {
				t[i][j] = 1 + t[i - 1][j - 1];
				best_count = max(t[i][j], best_count);
			}
			else
				t[i][j] = 0;

	int i = m, j = n;
	string output = "";

	while (i > 0 && j > 0) {
		if (a[i - 1] == b[i - 1]) {
			output.push_back(a[i - 1]);
			i--; j--;
		} else
			t[i][j - 1] > t[i - 1][j] ? j-- : i--;
	}
	reverse(output.begin(), output.end());

	return output;
}
```
